io/BeyondCriteria.ILangToMLang.fst
@@ -1,0 +1,109 @@
+module BeyondCriteria.ILangToMLang
+
+open FStar.Classical.Sugar
+open FStar.Tactics
+open FStar.List.Tot
+open FStar.Tactics.Typeclasses
+open FStar.FunctionalExtensionality
+
+open BeyondCriteria
+open RrHP
+
+type trace_property = (a:Type u#a & (Hist.hist_post #(IO.Sig.event) a))
+
+(**
+val _beh : (#a:Type u#a) -> (d:free a) ^-> trace_property u#a
+let _beh #a = 
+  on (free a) (fun d ->
+    (| a, (fun lt (r:a) -> forall p. IIO.dm_iio_theta d p [] ==> p lt r) |) <: trace_property)
+**)
+
+val _beh : (#a:Type u#a) -> (d:free.m a) -> trace_property u#a
+let _beh #a d = 
+    (| a, (fun lt (r:a) -> forall p. IIO.dm_iio_theta d p [] ==> p lt r) |)
+
+noeq type ilang_int = {
+  ctx_in : Type u#a; 
+  ctx_out : Type u#b; 
+  prog_out : Type u#c; 
+  vpi : pi_type; 
+}
+
+type ictx   (i:ilang_int) = x:i.ctx_in -> ILang.IIOpi i.ctx_out i.vpi
+type iprog  (i:ilang_int) = ictx i -> ILang.IIOpi i.prog_out i.vpi
+type iwhole = i:ilang_int & (unit -> ILang.IIOpi i.prog_out i.vpi)
+
+let ilink 
+  (#i:ilang_int) 
+  (ip:iprog i) 
+  (ic:ictx i) : 
+  iwhole = 
+  (| i, (fun () -> ip ic <: ILang.IIOpi i.prog_out i.vpi) |)
+
+val ibeh : iwhole u#a u#b u#c ^-> trace_property u#c
+let ibeh =
+  on (iwhole) (fun (| _, iw |) -> _beh (reify_IIOwp iw))
+
+let ilang : language trace_property = {
+  interface = ilang_int;
+  ctx   = ictx;
+  pprog = iprog;
+  whole = iwhole;
+  link  = ilink;
+  beh   = ibeh;
+}
+
+noeq type mlang_int = {
+  ctx_in : Type u#a; 
+  ctx_out : Type u#b; 
+  prog_out : Type u#c; 
+}
+
+type mctx   (i:mlang_int) = mon:monad -> acts mon -> i.ctx_in -> mon.m i.ctx_out
+type mprog  (i:mlang_int) = mctx i -> free.m i.prog_out
+type mwhole = i:mlang_int & (unit   -> free.m i.prog_out)
+
+let mlink 
+  (#i:mlang_int) 
+  (mp:mprog i) 
+  (mc:mctx i) : 
+  mwhole = 
+  (| i, (fun () -> mp mc) |)
+
+val mbeh : mwhole u#a u#b u#c ^-> trace_property u#c
+let mbeh =
+  on (mwhole) (fun (| _, mw |) -> _beh (mw ()))
+
+let mlang : language trace_property = {
+  interface = mlang_int;
+  ctx       = mctx;
+  pprog     = mprog;
+  whole     = mwhole;
+  link      = mlink;
+  beh       = mbeh;
+}
+
+let cint (i:ilang_int) : mlang_int = {
+  ctx_in = i.ctx_in;
+  ctx_out = i.ctx_out;
+  prog_out = i.prog_out;
+}
+
+let ilang_to_mlang : compiler trace_property = {
+  source = ilang;
+  target = mlang;
+  cint = cint;
+  compile_pprog = (fun #i sp -> 
+    compile_prog #i.vpi sp i.vpi #(r_pi i.vpi))
+}
+
+let bc_rrhc = BeyondCriteria.rrhc trace_property ilang_to_mlang
+let my_rrhc = forall i c. RrHP.rrhc i c
+
+let equivalence () : Lemma (bc_rrhc <==> my_rrhc) by (
+  explode ();
+  ExtraTactics.rewrite_lemma 2 3;
+  norm [delta_only [`%bc_rrhc; `%my_rrhc;`%BeyondCriteria.rrhc;`%RrHP.rrhc];iota];
+  explode ();
+  dump "H"
+)= ()
